Completed another refinement: explicit leadership acquisition.

Isabelle2/AbstractMultiPaxosR1.thy
@@ -3,11 +3,13 @@ AbstractMultiPaxosR1
 imports  "../../IO-Automata/IOA" BallotArrays3 DistributedSafeAt
 begin
 
-text {* 
+text {*
 1) Acceptors vote for a suggestion, and leaders use the distributed implementation of the safe-at computation.
 2) Explicit 1b messages.
 3) Explicit learning.
 4) Catch-up.
+5) Localizing suggestions (the leader function).
+6) Explicit leadership acquisition.
 *}
 
 type_synonym bal = nat
@@ -21,9 +23,11 @@ record ('v,'a,'l) amp_state =
   suggestion :: "inst \<Rightarrow> bal \<rightharpoonup> 'v"
   onebs :: "'a \<Rightarrow> bal \<rightharpoonup> (inst \<rightharpoonup> ('v\<times>bal))"
   learned :: "'l \<Rightarrow> inst \<rightharpoonup> 'v"
+  leader :: "'a \<Rightarrow> bool"
 
 locale amp_ioa = IOA +
-  fixes quorums::"'a set set"
+  fixes quorums::"'a set set" and leader :: "bal \<Rightarrow> 'a"
+  -- {* @{term leader} determines the leader of a ballot. *}
 begin
 
 datatype ('vv,'aa,'ll) amp_action =
@@ -40,7 +44,8 @@ definition amp_asig where
 definition amp_start where
   -- {* The initial state *}
   "amp_start \<equiv> {\<lparr>propCmd = {}, ballot = (\<lambda> a . 0), vote = (\<lambda> i a . Map.empty), 
-    suggestion = \<lambda> i . Map.empty, onebs = \<lambda> a . Map.empty, learned = \<lambda> l . Map.empty \<rparr>}"
+    suggestion = \<lambda> i . Map.empty, onebs = \<lambda> a . Map.empty, learned = \<lambda> l . Map.empty,
+    leader = \<lambda> a . leader 0 = a\<rparr>}"
 
 subsection {* The transitions *}
 
@@ -51,18 +56,28 @@ definition join_ballot where
   "join_ballot a b s s' \<equiv> 
     let onebs' = \<lambda> i . distributed_safe_at.acc_max (vote s i) a b
     in
-      b > (ballot s a) \<and> s' = s\<lparr>ballot := (ballot s)(a := b),
-        onebs := (onebs s)(a := (onebs s a)(b \<mapsto> onebs'))\<rparr>"
+      b > (ballot s a) 
+      \<and> s' = s\<lparr>ballot := (ballot s)(a := b),
+        onebs := (onebs s)(a := (onebs s a)(b \<mapsto> onebs')),
+        leader := (amp_state.leader s)(a := False)\<rparr>"
 
-definition suggest where
-  "suggest i b v q s s' \<equiv>
+definition acquire_leadership where
+  "acquire_leadership a q s s' \<equiv> let b = ballot s a in 
+    leader b = a
+    \<and> q \<in> quorums
+    \<and> \<not> amp_state.leader s a 
+    \<and> (\<forall> a \<in> q . onebs s a b \<noteq> None)
+    \<and> s' = s\<lparr>leader := (amp_state.leader s)(a := True), 
+        suggestion := \<lambda> i . (suggestion s i)(b := 
+          let m = distributed_safe_at.max_pair q (\<lambda> a . the (onebs s a b) i) in
+            map_option fst m)\<rparr>"
+
+definition suggest where "suggest a i b v s s' \<equiv>
           v \<in> propCmd s
+        \<and> ballot s a = b
+        \<and> amp_state.leader s a
         \<and> suggestion s i b = None
-        \<and> q \<in> quorums
-        \<and> (\<forall> a \<in> q . onebs s a b \<noteq> None)
-        \<and> (let m = distributed_safe_at.max_pair q (\<lambda> a . the (onebs s a b) i) in 
-            (case m of None \<Rightarrow> True | Some (v',b') \<Rightarrow> v = v')
-            \<and> s' = s\<lparr>suggestion := (suggestion s)(i := (suggestion s i)(b \<mapsto> v))\<rparr>)"
+        \<and> s' = s\<lparr>suggestion := (suggestion s)(i := (suggestion s i)(b \<mapsto> v))\<rparr>"
 
 definition do_vote where
   "do_vote a i v s s' \<equiv> let b = ballot s a in
@@ -85,8 +100,9 @@ fun amp_trans_rel where
 | "amp_trans_rel r Internal r' = (
     (\<exists> a b . join_ballot a b r r')
     \<or> (\<exists> a i v . do_vote a i v r r')
-    \<or> (\<exists> i b v q . suggest i b v q r r')
-    \<or> (\<exists> l1 l2 i v . catch_up l1 l2 i v r r'))"
+    \<or> (\<exists> a i b v . suggest a i b v r r')
+    \<or> (\<exists> l1 l2 i v . catch_up l1 l2 i v r r')
+    \<or> (\<exists> a q . acquire_leadership a q r r'))"
 | "amp_trans_rel r (Learn i v l) r' = learn l i v r r'"
 
 lemma trans_cases[consumes 1]:
@@ -96,8 +112,9 @@ lemma trans_cases[consumes 1]:
 | (learn) l i v where "learn l i v r r'"
 | (join_ballot) a b where "join_ballot a b r r'"
 | (do_vote) a i v where "do_vote a i v r r'"
-| (suggest) i b v q where "suggest i b v q r r'"
+| (suggest) a i b v where "suggest a i b v r r'"
 | (catch_up) l1 l2 i v where "catch_up l1 l2 i v r r'"
+| (acquire) a q where "acquire_leadership a q r r'"
 using assms by induct auto
 
 definition amp_trans where
